refactoring

clightDM/clightDM_mem/ClightlightMem1.v
@@ -12,13 +12,18 @@ From compcert Require Import Floats Integers Values Memory AST Ctypes Clight Cli
 
 Set Implicit Arguments.
 
-Let _memcntRA: URA.t := (block ==> Z ==> (Excl.t (permission * permission * memval)))%ra.
-Let _memszRA: URA.t := (block ==> (Excl.t Z))%ra.
+Inductive block_kind :=
+| Dynamic
+| Local
+| Unfreeable.
+
+Let _memcntRA: URA.t := (block ==> Z ==> (Consent.t memval))%ra.
+Let _memhdRA: URA.t := (block ==> (Excl.t (Z * block_kind)))%ra.
 
 Compute (URA.car (t:=_memcntRA)).
-Compute (URA.car (t:=_memszRA)).
+Compute (URA.car (t:=_memhdRA)).
 Instance memcntRA: URA.t := Auth.t _memcntRA.
-Instance memszRA: URA.t := Auth.t _memszRA.
+Instance memhdRA: URA.t := Auth.t _memhdRA.
 
 Section RA.
 
@@ -26,30 +31,22 @@ Section POINTSTO.
 
   Local Open Scope Z.
 
-  Definition __points_to (b: block) (ofs: Z) (p_cur: permission) (p_max: permission) (mvs: list memval): _memcntRA :=
+  Definition __points_to (b: block) (ofs: Z) (mvs: list memval) (q: Qp): _memcntRA :=
     (fun _b _ofs => if (dec _b b) && ((Coqlib.zle ofs _ofs) && (Coqlib.zlt _ofs (ofs + Z.of_nat (List.length mvs))))
                     then 
                       match List.nth_error mvs (Z.to_nat (_ofs - ofs)) with
-                      | Some mv => Some (p_cur, p_max, mv)
+                      | Some mv => Consent.just q mv
                       | None => ε
                       end
                     else ε)
   .
 
-  (* Opaque _points_to. *)
-  (* Lemma unfold__points_to b ofs vs:
-    __points_to b ofs vs =
-    (fun _b _ofs => if (dec _b b) && ((ofs <=? _ofs) && (_ofs <? (ofs + Z.of_nat (List.length vs))))%Z
-                    then (List.nth_error vs (Z.to_nat (_ofs - ofs))) else ε)
-  .
-  Proof. refl. Qed. *)
-
-  Definition _points_to (b: block) (ofs: Z) (p_cur: permission) (p_max: permission) (mvs: list memval): memcntRA := Auth.white (__points_to b ofs p_cur p_max mvs).
+  Definition _points_to (b: block) (ofs: Z) (mvs: list memval) (q: Qp): memcntRA := Auth.white (__points_to b ofs mvs q).
 
   Lemma _points_to_split_aux
-        blk ofs hd tl p_cur p_max
+        blk ofs hd tl q
     :
-      (_points_to blk ofs p_cur p_max (hd :: tl)) = (_points_to blk ofs p_cur p_max [hd]) ⋅ (_points_to blk (ofs + 1)%Z p_cur p_max tl)
+      (_points_to blk ofs (hd :: tl) q) = (_points_to blk ofs [hd] q) ⋅ (_points_to blk (ofs + 1)%Z tl q)
   .
   Proof.
     ss. unfold _points_to, Auth.white. repeat (rewrite URA.unfold_add; ss).
@@ -79,20 +76,20 @@ Section POINTSTO.
       rewrite Z.sub_add_distr in *. rewrite Z2Nat.inj_sub in Heq4; ss. rewrite T in *. ss. rewrite Nat.sub_0_r in *. ss. clarify.
   Qed.
 
-  Lemma __points_to_nil : forall blk ofs p_cur p_max _b _ofs, __points_to blk ofs p_cur p_max [] _b _ofs = ε.
+  Lemma __points_to_nil : forall blk ofs q _b _ofs, __points_to blk ofs [] _b _ofs q = ε.
   Proof.
     intros. unfold __points_to. ss. des_ifs. destruct (Z.to_nat _) in Heq0; ss. 
   Qed.
 
-  Lemma points_to_nil : forall blk ofs p_cur p_max, _points_to blk ofs p_cur p_max [] = ε.
+  Lemma points_to_nil : forall blk ofs q, _points_to blk ofs [] q = ε.
   Proof.
     intros. ss. unfold _points_to, Auth.white.
     change (memcntRA.(URA.unit)) with (Auth.frag (_memcntRA.(URA.unit))). f_equal. ss.
     repeat (apply func_ext; i). apply __points_to_nil.
   Qed.
 
-  Lemma _points_to_app l l' p_cur p_max blk ofs:
-    (_points_to blk ofs p_cur p_max (l++l')) = (_points_to blk ofs p_cur p_max l) ⋅ (_points_to blk (ofs + length l) p_cur p_max l').
+  Lemma _points_to_app l l' q blk ofs:
+    (_points_to blk ofs (l++l') q) = (_points_to blk ofs l q) ⋅ (_points_to blk (ofs + length l) l' q).
   Proof.
     revert l' blk ofs. induction l;i;ss.
     - rewrite points_to_nil. rewrite URA.unit_idl. rewrite Z.add_0_r. auto.
@@ -103,9 +100,9 @@ Section POINTSTO.
   Qed.
 
   Lemma _points_to_split :
-    forall (blk : Values.block) (ofs : Z) (p_cur: permission) (p_max: permission) (n : nat) (l : list memval),
-      _points_to blk ofs p_cur p_max l =
-        _points_to blk ofs p_cur p_max (firstn n l) ⋅ _points_to blk (ofs + (length (firstn n l))) p_cur p_max (skipn n l).
+    forall (blk : Values.block) (ofs : Z) (q: Qp) (n : nat) (l : list memval),
+      _points_to blk ofs l q =
+        _points_to blk ofs (firstn n l) q ⋅ _points_to blk (ofs + (length (firstn n l))) (skipn n l) q.
   Proof.
     intros. set l as k at 2 3 4. rewrite <- (firstn_skipn n l). unfold k. clear k.
     rewrite _points_to_app. auto.
@@ -113,32 +110,33 @@ Section POINTSTO.
 
 End POINTSTO.
 
-Section SZOF.
+Section ALLOCEDWITH.
 
-  Definition __sz_of (b: block) (sz: Z) : _memszRA :=
+  Definition __alloced_with (b: block) (sz: Z) (bk: block_kind) : _memhdRA :=
     (fun _b => if dec _b b
-               then Excl.just sz
+               then Excl.just (sz, bk)
                else ε)
   .
 
-  Definition _sz_of (b: block) (sz: Z) : memszRA := Auth.white (__sz_of b sz).
+  Definition _alloced_with (b: block) (sz: Z) (bk: block_kind) : memhdRA := Auth.white (__alloced_with b sz bk).
 
-End SZOF.
+End ALLOCEDWITH.
 
 End RA.
 
 Section PROP.
 
   Context `{@GRA.inG memcntRA Σ}.
-  Context `{@GRA.inG memszRA Σ}.
+  Context `{@GRA.inG memhdRA Σ}.
 
-  Definition updblk [A: Type] (i f: nat) (l l': list A) : list A := firstn i l ++ l' ++ skipn f l.
+  (* Definition updblk [A: Type] (i f: nat) (l l': list A) : list A := firstn i l ++ l' ++ skipn f l.
   Definition getblk [A: Type] (i delta: nat) (l: list A) : list A := firstn delta (skipn i l).
 
+  (* how to use getblk, updblk *)
   Lemma getblk_updblk A (i delta: nat) (l: list A) : updblk i (i + delta) l (getblk i delta l) = l.
   Proof.
     unfold updblk, getblk. rewrite <- drop_drop. do 2 rewrite firstn_skipn. refl.
-  Qed.
+  Qed. *)
 
   Definition size_rule (sz: nat) : Z :=
     if sz <? 2 then 1
@@ -147,33 +145,24 @@ Section PROP.
     else 8
   .
 
-  Definition points_to addr p_cur p_max mvs : iProp :=
+  Definition points_to addr mvs q : iProp :=
     match addr with
     | Vptr b ofs =>
           let ofs' := Ptrofs.unsigned ofs in
           let align := size_rule (Z.to_nat (length mvs)) in
-          OwnM (_points_to b ofs' p_cur p_max mvs)
-          ** ⌜(align | ofs') /\ perm_order p_cur p_max⌝
-    | _ => ⌜False⌝%I 
-    end.
-
-  Definition mpoints_to addr sz mvs : iProp :=
-    match addr with
-    | Vptr b ofs =>
-          let ofs' := Ptrofs.unsigned ofs in
-          let align := size_rule (Z.to_nat sz) in
-          OwnM (_points_to b ofs' Freeable Freeable mvs) ** OwnM (_sz_of b sz)
+          OwnM (_points_to b ofs' mvs q)
           ** ⌜(align | ofs')⌝
     | _ => ⌜False⌝%I 
     end.
+  
+  Definition alloced_with b sz bk : iProp :=
+    OwnM (_alloced_with b sz bk).
 
-  Definition has_addr v b ofs : iProp :=
+  Definition has_ofs v b ofs : iProp :=
     match v with
     | Vptr b' ofs' => ⌜b' = b /\ Ptrofs.unsigned ofs' = ofs⌝%I
     | _ => ⌜False⌝%I 
     end.
-
-  Definition allocated b sz : iProp := OwnM (_sz_of b sz).
 
   (* Lemma detach_size addr vs sz : (addr #↦ vs ⋯ sz) -∗ (addr ↦ vs).
   Proof. 
@@ -220,8 +209,8 @@ Section PROP.
 
 End PROP.
 
-Notation "addr ↦ ( p_cur , p_max , mvs )" := (points_to addr p_cur p_max mvs) (at level 20).
-Notation "addr #↦ vs ⋯ sz" := (mpoints_to addr sz vs) (at level 10).
+Notation "addr |_ q #> mvs" := (points_to addr mvs q) (at level 20).
+Notation "b #≔ ( sz , bk )" := (alloced_with b sz bk) (at level 10).
 
 Section AUX.
 
@@ -293,7 +282,7 @@ End AUX.
 Section SMODSEM.
 
   Context `{@GRA.inG memcntRA Σ}.
-  Context `{@GRA.inG memszRA Σ}.
+  Context `{@GRA.inG memhdRA Σ}.
 
   Variable sk: Sk.t.
   Let skenv: SkEnv.t := Sk.load_skenv sk.
@@ -307,64 +296,76 @@ Section SPEC.
     (mk_simple (fun sz => (
                     (ord_pure 0%nat),
                     (fun varg => ⌜varg = sz↑⌝),
-                    (fun vret => ∃ b addr, ⌜vret = b↑⌝
-                                 ** addr ↦ (Freeable, Freeable, List.repeat Undef (Z.to_nat sz))
-                                 ** has_addr addr b 0)
+                    (fun vret => ∃ b vaddr, ⌜vret = b↑⌝
+                                 ** vaddr |_1#> List.repeat Undef (Z.to_nat sz)
+                                 ** b #≔ (sz, Local)
+                                 ** has_ofs vaddr b 0)
     )))%I.
 
   Definition sfree_spec: fspec :=
     (mk_simple (fun '() => (
                    (ord_pure 0%nat),
-                   (fun varg => ∃ mvl addr b sz, ⌜varg = (b, sz)↑ /\ Z.of_nat (List.length mvl) = sz⌝
-                                ** addr ↦ (Freeable, Freeable, mvl)
-                                ** has_addr addr b 0),
+                   (fun varg => ∃ mvl vaddr b sz,
+                                ⌜varg = (b, sz)↑ /\ Z.of_nat (List.length mvl) = sz⌝
+                                ** vaddr |_1#> mvl
+                                ** b #≔ (sz, Local)
+                                ** has_ofs vaddr b 0),
                    (fun vret => ⌜vret = tt↑⌝)
     )))%I.
 
   Definition load_spec: fspec :=
-    (mk_simple (fun '(chunk, addr, p_cur, p_max, l) => (
+    (mk_simple (fun '(chunk, vaddr, q, mvs) => (
                     (ord_pure 0%nat),
-                    (fun varg => ⌜varg = (chunk, addr)↑ /\ perm_order Readable p_cur⌝ ** addr ↦ (p_cur, p_max, l)),
-                    (fun vret => ∃ v, ⌜vret = v↑ /\ decode_val chunk l = v⌝ ** addr ↦ (p_cur, p_max, l))
+                    (fun varg => ⌜varg = (chunk, vaddr)↑⌝
+                                 ** vaddr |_q#> mvs),
+                    (fun vret => ∃ v, ⌜vret = v↑ /\ decode_val chunk mvs = v⌝
+                                 ** vaddr |_q#> mvs)
     )))%I.
 
   Definition loadbytes_spec: fspec :=
-    (mk_simple (fun '(addr, p_cur, p_max, n, l) => (
+    (mk_simple (fun '(vaddr, sz, q, mvs) => (
                     (ord_pure 0%nat),
-                    (fun varg => ⌜varg = (addr, n)↑ /\ Z.of_nat (List.length l) = n /\ perm_order Readable p_cur⌝ 
-                                 ** addr ↦ (p_cur, p_max, l)),
-                    (fun vret => ⌜vret = l↑⌝ ** addr ↦ (p_cur, p_max, l))
+                    (fun varg => ⌜varg = (vaddr, sz)↑ /\ Z.of_nat (List.length mvs) = sz⌝ 
+                                 ** vaddr |_q#> mvs),
+                    (fun vret => ⌜vret = mvs↑⌝ ** vaddr |_q#> mvs)
     ))).
 
   Definition store_spec: fspec :=
     (mk_simple
-       (fun '(chunk, addr, p_cur, p_max, v_new) => (
+       (fun '(chunk, vaddr, v_new) => (
             (ord_pure 0%nat),
-            (fun varg => ∃ l_old, ⌜varg = (chunk, addr, v_new)↑ /\ List.length l_old = size_chunk_nat chunk 
-                         /\ perm_order Writable p_cur⌝
-                         ** addr ↦ (p_cur, p_max, l_old)),
-            (fun vret => ∃ l_new, ⌜vret = tt↑ /\ encode_val chunk v_new = l_new⌝
-                         ** addr ↦ (p_cur, p_max, l_new))
+            (fun varg => ∃ mvs_old, ⌜varg = (chunk, vaddr, v_new)↑
+                                    /\ List.length mvs_old = size_chunk_nat chunk⌝
+                                    ** vaddr |_1#> mvs_old),
+            (fun vret => ∃ mvs_new, ⌜vret = tt↑ /\ encode_val chunk v_new = mvs_new⌝
+                                    ** vaddr |_1#> mvs_new)
     )))%I.
 
   Definition storebytes_spec: fspec :=
     (mk_simple
-       (fun '(addr, p_cur, p_max, l_new) => (
+       (fun '(vaddr, mvs_new) => (
             (ord_pure 0%nat),
-            (fun varg => ∃ l_old, ⌜varg = (addr, l_new)↑ /\ List.length l_old = List.length l_new /\ perm_order p_cur Writable⌝
-                         ** addr ↦ (p_cur, p_max, l_old)),
-            (fun vret => ⌜vret = tt↑⌝ ** addr ↦ (p_cur, p_max, l_new))
+            (fun varg => ∃ mvs_old, ⌜varg = (vaddr, mvs_new)↑
+                                    /\ List.length mvs_old = List.length mvs_new⌝
+                                    ** vaddr |_1#> mvs_old),
+            (fun vret => ⌜vret = tt↑⌝ ** vaddr |_1#> mvs_new)
     )))%I.
+  
+  Definition is_valid (res: Excl.t (Z * block_kind)) (ofs: Z) : bool :=
+    match res with
+    | Excl.just (sz, _) => Coqlib.zle 0 ofs && Coqlib.zlt ofs sz
+    | _ => false
+    end.
 
   Definition valid_pointer_spec: fspec :=
     (mk_simple
-       (fun '(result, iprop) => (
+       (fun '(b, ofs, resource) => (
             (ord_pure 0%nat),
-            (fun varg =>
-            ((∃ addr p_cur p_max mvl, ⌜varg = addr↑ /\ iprop = (addr ↦ (p_cur, p_max, mvl)) /\ result = true⌝) ∨
-                (∃ addr p_cur p_max mvl, ⌜varg = addr↑ /\ iprop <> (addr ↦ (p_cur, p_max, mvl)) /\ result = false⌝))
-                ** iprop),
-            (fun vret => ⌜vret = result↑⌝ ** iprop)%I
+            (fun varg => ∃ vaddr, ⌜varg = vaddr↑⌝
+                         ** has_ofs vaddr b ofs
+                         ** OwnM (Auth.white resource)),
+            (fun vret => ⌜vret = (is_valid (resource b) ofs)↑⌝ 
+                         ** OwnM (Auth.white resource))%I
     )))%I.
 
   (* heap malloc free *)
@@ -372,17 +373,20 @@ Section SPEC.
     (mk_simple (fun sz => (
                     (ord_pure 0%nat),
                     (fun varg => ⌜varg = (Vptrofs sz)↑⌝),
-                    (fun vret => ∃ addr b, ⌜vret = addr↑⌝
-                                 ** addr #↦ List.repeat Undef (Z.to_nat (Ptrofs.unsigned sz)) ⋯ (Ptrofs.unsigned sz)
-                                 ** has_addr addr b 0) 
+                    (fun vret => ∃ vaddr b, ⌜vret = vaddr↑⌝
+                                 ** vaddr |_1#> List.repeat Undef (Z.to_nat (Ptrofs.unsigned sz))
+                                 ** b #≔ (Ptrofs.unsigned sz, Dynamic)
+                                 ** has_ofs vaddr b 0) 
     )))%I.
 
   Definition mfree_spec: fspec :=
     (mk_simple (fun '() => (
                     (ord_pure 0%nat),
-                    (fun varg => ∃ mvl addr b sz, ⌜varg = addr↑ /\ Z.of_nat (List.length mvl) = sz⌝
-                                 ** addr #↦ mvl ⋯ sz
-                                 ** has_addr addr b 0),
+                    (fun varg => ∃ mvs vaddr b sz,
+                                 ⌜varg = vaddr↑ /\ Z.of_nat (List.length mvs) = sz⌝
+                                 ** vaddr |_1#> mvs
+                                 ** b #≔ (sz, Dynamic)
+                                 ** has_ofs vaddr b 0),
                     (fun vret => ⌜vret = tt↑⌝)
     )))%I.
 
@@ -419,60 +423,108 @@ End SPECBODY.
 
 Section MRS.
 
-  (* have to make predicate, need to restrict alignment. *)
-  Definition store_init_data (res : _memcntRA) (b : block) (p : Z) (perm : permission) (id : init_data) :=
+  Definition store_init_data (res : _memcntRA) (b : block) (p : Z) (optq : option Qp) (id : init_data) : option _memcntRA :=
     match id with
     | Init_int8 n => 
-      if Zdivide_dec 1 p then Some (__points_to b p perm perm (encode_val Mint8unsigned (Vint n)) ⋅ res)
+      if Zdivide_dec (align_chunk Mint8unsigned) p
+      then
+        match optq with
+        | Some q => Some (__points_to b p (encode_val Mint8unsigned (Vint n)) q ⋅ res)
+        | None => Some res
+        end
       else None
     | Init_int16 n =>
-      if Zdivide_dec 2 p then Some (__points_to b p perm perm (encode_val Mint16unsigned (Vint n)) ⋅ res )
+      if Zdivide_dec (align_chunk Mint16unsigned) p
+      then
+        match optq with
+        | Some q => Some (__points_to b p (encode_val Mint16unsigned (Vint n)) q ⋅ res)
+        | None => Some res
+        end
       else None
     | Init_int32 n =>
-      if Zdivide_dec 4 p then Some (__points_to b p perm perm (encode_val Mint32 (Vint n)) ⋅ res)
+      if Zdivide_dec (align_chunk Mint32) p
+      then
+        match optq with
+        | Some q => Some (__points_to b p (encode_val Mint32 (Vint n)) q ⋅ res)
+        | None => Some res
+        end
       else None
     | Init_int64 n =>
-      if Zdivide_dec 8 p then Some (__points_to b p perm perm (encode_val Mint64 (Vlong n)) ⋅ res)
+      if Zdivide_dec (align_chunk Mint64) p
+      then
+        match optq with
+        | Some q => Some (__points_to b p (encode_val Mint64 (Vlong n)) q ⋅ res)
+        | None => Some res
+        end
       else None
     | Init_float32 n =>
-      if Zdivide_dec 4 p then Some (__points_to b p perm perm (encode_val Mfloat32 (Vsingle n)) ⋅ res)
+      if Zdivide_dec (align_chunk Mfloat32) p
+      then
+        match optq with
+        | Some q => Some (__points_to b p (encode_val Mfloat32 (Vsingle n)) q ⋅ res)
+        | None => Some res
+        end
       else None
     | Init_float64 n =>
-      if Zdivide_dec 4 p then Some (__points_to b p perm perm (encode_val Mfloat64 (Vfloat n)) ⋅ res)
-      else None
-    | Init_space z => Some (__points_to b p perm perm (repeat (Byte Byte.zero) (Z.to_nat z))  ⋅ res)
-    | Init_addrof symb ofs =>
-        match SkEnv.id2blk skenv (string_of_ident symb) with
-        | Some b' =>
-          if Zdivide_dec (if Archi.ptr64 then 8 else 4) p then Some (__points_to b p perm perm (encode_val Mptr (Vptr (Pos.of_succ_nat b') ofs)) ⋅ res)
-          else None
-        | None => None
+      if Zdivide_dec (align_chunk Mfloat64) p
+      then
+        match optq with
+        | Some q => Some (__points_to b p (encode_val Mfloat64 (Vfloat n)) q ⋅ res)
+        | None => Some res
         end
+      else None
+    | Init_space z => 
+      match optq with
+      | Some q => Some (__points_to b p (repeat (Byte Byte.zero) (Z.to_nat z)) q ⋅ res)
+      | None => Some res
+      end
+    | Init_addrof symb ofs =>
+      match SkEnv.id2blk skenv (string_of_ident symb) with
+      | Some b' =>
+        if Zdivide_dec (align_chunk Mptr) p
+        then
+          match optq with
+          | Some q => Some (__points_to b p (encode_val Mptr (Vptr (Pos.of_succ_nat b') ofs)) q ⋅ res)
+          | None => Some res
+          end
+        else None
+      | None => None
+      end
     end.
 
-  Fixpoint store_init_data_list (res : _memcntRA) (b : block) (p : Z) (perm: permission) (idl : list init_data) {struct idl} : option _memcntRA :=
+  Fixpoint store_init_data_list (res : _memcntRA) (b : block) (p : Z) (optq: option Qp) (idl : list init_data) {struct idl} : option _memcntRA :=
     match idl with
     | [] => Some res
     | id :: idl' =>
-        match store_init_data res b p perm id with
-        | Some res' => store_init_data_list res' b (p + init_data_size id)%Z perm idl'
+        match store_init_data res b p optq id with
+        | Some res' => store_init_data_list res' b (p + init_data_size id)%Z optq idl'
         | None => None
         end
     end.
-  
 
-  Definition alloc_global (res : _memcntRA) (b: block) (entry : string * Any.t) :=
+  Definition alloc_global (res : Σ) (b: block) (entry : string * Any.t) : option Σ :=
     let (_, agd) := entry in
     match Any.downcast agd : option (globdef Clight.fundef type) with
     | Some g => 
       match g with
-      | Gfun _ => Some (__points_to b 0 Nonempty Nonempty [Undef] ⋅ res)
-      | Gvar v => store_init_data_list res b 0 (Globalenvs.Genv.perm_globvar v) (gvar_init v)
+      | Gfun _ => Some (GRA.embed (Auth.black (__alloced_with b 1 Unfreeable)) ⋅ res)
+      | Gvar v =>
+        let optq := match Globalenvs.Genv.perm_globvar v with
+                    | Freeable | Writable => Some 1%Qp
+                    | Readable => Some (1/2)%Qp
+                    | Nonempty => None
+                    end
+        in
+        match store_init_data_list ε b 0 optq (gvar_init v) with
+        | Some res' => Some (GRA.embed (Auth.black (__alloced_with b (init_data_list_size (gvar_init v)) Unfreeable))
+                             ⋅ GRA.embed (Auth.black res') ⋅ res)
+        | None => None
+        end
       end
     | None => None
     end.
 
-  Fixpoint alloc_globals (res: _memcntRA) (b: block) (sk: list (string * Any.t)) : _memcntRA :=
+  Fixpoint alloc_globals (res: Σ) (b: block) (sk: list (string * Any.t)) : Σ :=
   match sk with
   | nil => res
   | g :: gl' => 
@@ -482,22 +534,23 @@ Section MRS.
     end
   end.
 
-  Definition load_mem := alloc_globals ε xH sk.
+  Definition load_resource : Σ := alloc_globals ε xH sk.
 
   End MRS.
 
   Definition SMemSem : SModSem.t := {|
     SModSem.fnsems := MemSbtb;
     SModSem.mn := "Mem";
-    SModSem.initial_mr := GRA.embed (Auth.black load_mem) ⋅ GRA.embed (Auth.black _memszRA.(URA.unit));
+    SModSem.initial_mr := load_resource;
     SModSem.initial_st := tt↑;
   |}
   .
+
   End SMODSEM.
 
 Section MOD.
   Context `{@GRA.inG memcntRA Σ}.
-  Context `{@GRA.inG memszRA Σ}.
+  Context `{@GRA.inG memhdRA Σ}.
 
   Definition SMem: SMod.t := {|
     SMod.get_modsem := SMemSem;
@@ -513,4 +566,4 @@ End MOD.
 Global Hint Unfold MemStb: stb.
 
 Global Opaque _points_to.
-Global Opaque _sz_of.
+Global Opaque _alloced_with.
