clight_examples/prooflib/PtrofsArith.v
@@ -1,0 +1,195 @@
+Require Import Coqlib.
+From compcert Require Import Integers Ctypes.
+Require Import ConvC2ITree.
+
+#[global] Transparent Ptrofs.repr.
+
+Lemma modulus_non_zero: Ptrofs.modulus <> 0%Z.
+Proof.
+  unfold Ptrofs.modulus.
+  unfold Ptrofs.wordsize.
+  unfold Wordsize_Ptrofs.wordsize.
+  destruct (Archi.ptr64); intro; inversion H.
+Qed.
+
+Lemma mul_modulus: forall x y,
+Ptrofs.Z_mod_modulus
+  (Ptrofs.Z_mod_modulus x * Ptrofs.Z_mod_modulus y)
+= Ptrofs.Z_mod_modulus (x * y).
+Proof.
+  intros.
+  repeat (rewrite Ptrofs.Z_mod_modulus_eq).
+  symmetry.
+  apply Z.mul_mod.
+  apply modulus_non_zero.
+Qed.
+
+Lemma mul_modulus_l: forall x y,
+Ptrofs.Z_mod_modulus
+  (Ptrofs.Z_mod_modulus x * y)
+= Ptrofs.Z_mod_modulus (x * y).
+Proof.
+  intros.
+  repeat (rewrite Ptrofs.Z_mod_modulus_eq).
+  apply Z.mul_mod_idemp_l.
+  apply modulus_non_zero.
+Qed.
+
+Lemma mul_modulus_r: forall x y,
+Ptrofs.Z_mod_modulus
+  (x * Ptrofs.Z_mod_modulus y)
+= Ptrofs.Z_mod_modulus (x * y).
+Proof.
+  intros.
+  repeat (rewrite Ptrofs.Z_mod_modulus_eq).
+  apply Z.mul_mod_idemp_r.
+  apply modulus_non_zero.
+Qed.
+
+Lemma add_modulus: forall x y,
+Ptrofs.Z_mod_modulus
+  (Ptrofs.Z_mod_modulus x + Ptrofs.Z_mod_modulus y)
+= Ptrofs.Z_mod_modulus (x + y).
+Proof.
+  intros.
+  repeat (rewrite Ptrofs.Z_mod_modulus_eq).
+  symmetry.
+  apply Zplus_mod.
+Qed.
+
+Lemma add_modulus_l: forall x y,
+Ptrofs.Z_mod_modulus
+  (Ptrofs.Z_mod_modulus x + y)
+= Ptrofs.Z_mod_modulus (x + y).
+Proof.
+  intros.
+  repeat (rewrite Ptrofs.Z_mod_modulus_eq).
+  apply Z.add_mod_idemp_l.
+  apply modulus_non_zero.
+Qed.
+
+Lemma add_modulus_r: forall x y,
+Ptrofs.Z_mod_modulus
+  (x + Ptrofs.Z_mod_modulus y)
+= Ptrofs.Z_mod_modulus (x + y).
+Proof.
+  intros.
+  repeat (rewrite Ptrofs.Z_mod_modulus_eq).
+  apply Z.add_mod_idemp_r.
+  apply modulus_non_zero.
+Qed.
+
+Lemma Zbits_p_mod_two_p_trivial: forall (x: positive),
+  (Zpos x < two_power_nat 32)%Z ->
+  Zbits.P_mod_two_p x (if Archi.ptr64 then 64%nat else 32%nat) = Zpos x.
+Proof.
+  intros.
+  rewrite Zbits.P_mod_two_p_eq.
+  destruct Archi.ptr64.
+  - apply Z.mod_small.
+    split.
+    + lia.
+    + assert (two_power_nat 32 < two_power_nat 64)%Z by reflexivity.
+      lia.
+  - apply Z.mod_small.
+    lia.
+Qed.
+
+Lemma mod_modulus_idempotent: forall x, Ptrofs.Z_mod_modulus (Ptrofs.Z_mod_modulus x) = Ptrofs.Z_mod_modulus x.
+ intro.
+ repeat (rewrite Ptrofs.Z_mod_modulus_eq).
+ apply (Z.mod_mod).
+ apply modulus_non_zero.
+Qed.
+
+Create HintDb Ptrofs_arith.
+
+#[export] Hint Unfold
+  Ptrofs.repr
+  Ptrofs.add
+  Ptrofs.mul
+  align_attr
+  bitalignof
+  Coqlib.align
+  bitsizeof
+  align_attr
+  sizeof_struct
+  bytes_of_bits
+  Ptrofs.modulus
+  Ptrofs.wordsize
+  Wordsize_Ptrofs.wordsize
+: Ptrofs_arith.
+
+#[export] Hint Rewrite
+  Ptrofs.Z_mod_modulus_eq
+  Zbits_p_mod_two_p_trivial
+: Ptrofs_arith.
+
+Ltac Zify.zify_post_hook ::= Z.div_mod_to_equations.
+
+Ltac solve_ptr_eq :=
+  repeat match goal with
+  | H:= hide |- _ => try clear H end;
+  apply Ptrofs.mkint_eq;
+  repeat (autounfold with Ptrofs_arith; autorewrite with Ptrofs_arith;
+  simpl);
+  destruct (Archi.ptr64);
+  simpl;
+  unfold two_power_nat;
+  simpl;
+  zify;
+  lia.
+(*
+Ltac rewrite_ptrofs ptr1 ptr2 :=
+  let H1 := fresh in
+  let H2 := fresh in
+  let H2eq := fresh in
+  assert (H1: ptr1 = ptr2);
+  [apply Ptrofs.mkint_eq;
+  repeat (autounfold with Ptrofs_arith;
+  simpl);
+  repeat rewrite Ptrofs.Z_mod_modulus_eq;
+  unfold Ptrofs.modulus;
+  unfold Ptrofs.wordsize;
+  unfold Wordsize_Ptrofs.wordsize;
+  destruct (Archi.ptr64);
+  simpl;
+  [remember (two_power_nat 64) as H2 eqn: H2eq;
+  vm_compute in H2eq; rewrite H2eq|
+  remember (two_power_nat 32) as H2 eqn: H2eq;
+  vm_compute in H2eq; rewrite H2eq];
+  simpl;
+  zify;
+  lia
+  | rewrite H1; clear H1].
+
+Ltac simpl_ptrofs ptr :=
+  match goal with
+  | [|- gpaco8 _ _ _ _ _ _ _ _ _ _ _ ?x] =>
+    let H := fresh in
+    pose (H := x);
+    match goal with
+    | [_ := context[Ptrofs.repr ?t] |- _] => rewrite_ptrofs (Ptrofs.repr t) ptr
+    | [_ := context[Ptrofs.add ?t1 ?t2] |- _] => rewrite_ptrofs (Ptrofs.add t1 t2) ptr
+    | [_ := context[Ptrofs.mul ?t1 ?t2] |- _] => rewrite_ptrofs (Ptrofs.mul t1 t2) ptr
+    end;
+    clear H
+  end.
+
+#[export] Hint Rewrite
+  mul_modulus
+  mul_modulus_l
+  mul_modulus_r
+  add_modulus
+  add_modulus_l
+  add_modulus_r
+  Z.add_0_r
+  Z.add_0_l
+  Zbits_p_mod_two_p_trivial
+  mod_modulus_idempotent
+  using reflexivity
+: Ptrofs_arith.
+
+Ltac red_ptrofs H :=
+  repeat (autounfold with Ptrofs_arith; simpl; autorewrite with Ptrofs_arith).
+*)
